deps/poulet4/lib/P4cub/Semantics/Static/Auxiliary.v
@@ -3,6 +3,7 @@ From Poulet4 Require Export
      P4cub.Semantics.Static.Typing
      P4cub.Semantics.Static.IndPrincip
      P4cub.Semantics.Static.Util
+     P4cub.Syntax.Shift
      Utils.ForallMap.
 
 Ltac inv_numeric_width :=
@@ -26,47 +27,8 @@ Ltac invert_type_lists_ok :=
   end.
 
 Section Lemmas.
-  Local Hint Resolve type_lists : core.
-  Local Hint Constructors type_lists_ok : core.
-  Local Hint Constructors t_ok_lists : core.
-
-  Lemma type_array : forall Δ Γ τ es,
-      t_ok Δ τ ->
-      Forall (fun e => `⟨ Δ, Γ ⟩ ⊢ e ∈ τ) es ->
-      `⟨ Δ, Γ ⟩ ⊢ Expr.Lists (Expr.lists_array τ) es
-        ∈ Expr.TArray (N.of_nat (length es)) τ.
-  Proof.
-    intros D G t es tok Hes; econstructor; eauto.
-    rewrite Nnat.Nat2N.id.
-    auto using Forall2_repeat_r.
-  Qed.
-
-  Lemma type_struct : forall Δ Γ es τs,
-      Forall2 (type_expr Δ Γ) es τs ->
-      `⟨ Δ, Γ ⟩ ⊢ Expr.Lists Expr.lists_struct es ∈ Expr.TStruct false τs.
-  Proof. eauto. Qed.
-
-  Lemma type_header : forall Δ Γ b es τs,
-      Forall2 (type_expr Δ Γ) es τs ->
-      `⟨ Δ, Γ ⟩ ⊢ Expr.Lists (Expr.lists_header b) es ∈ Expr.TStruct true τs.
-  Proof. eauto. Qed.
-
   Local Hint Constructors t_ok : core.
   
-  Lemma type_expr_t_ok : forall Δ Γ e τ,
-      `⟨ Δ, Γ ⟩ ⊢ e ∈ τ ->
-      Forall (t_ok Δ) Γ ->
-      t_ok Δ τ.
-  Proof.
-    intros D G e t het hok;
-      induction het using custom_type_expr_ind; auto.
-    apply Forall2_only_r_Forall in H2.
-    rewrite Forall_forall in H2.
-    pose proof (fun t hin => H2 t hin hok) as h; clear H2.
-    rewrite <- Forall_forall in h.
-    inv H; inv H0; auto.
-  Qed.
-
   Lemma t_ok_le : forall Δ₁ Δ₂ τ,
       (Δ₁ <= Δ₂)%nat -> t_ok Δ₁ τ -> t_ok Δ₂ τ.
   Proof.
@@ -79,4 +41,90 @@ Section Lemmas.
   Lemma t_ok_0 : forall Δ τ,
       t_ok 0 τ -> t_ok Δ τ.
   Proof. intros n t; apply t_ok_le; lia. Qed.
+  
+  Local Hint Resolve type_lists : core.
+  Local Hint Constructors type_lists_ok : core.
+  Local Hint Constructors t_ok_lists : core.
+
+  Variable Δ : nat.
+  Variable Γ : list Expr.t.
+
+  Lemma type_expr_t_ok : forall e τ,
+      `⟨ Δ, Γ ⟩ ⊢ e ∈ τ ->
+      Forall (t_ok Δ) Γ ->
+      t_ok Δ τ.
+  Proof using.
+    intros e t het hok;
+      induction het using custom_type_expr_ind; auto.
+    apply Forall2_only_r_Forall in H2.
+    rewrite Forall_forall in H2.
+    pose proof (fun t hin => H2 t hin hok) as h; clear H2.
+    rewrite <- Forall_forall in h.
+    inv H; inv H0; auto.
+  Qed.
+  
+  Lemma type_array : forall τ es,
+      t_ok Δ τ ->
+      Forall (fun e => `⟨ Δ, Γ ⟩ ⊢ e ∈ τ) es ->
+      `⟨ Δ, Γ ⟩ ⊢ Expr.Lists (Expr.lists_array τ) es
+        ∈ Expr.TArray (N.of_nat (length es)) τ.
+  Proof using.
+    intros t es tok Hes; econstructor; eauto.
+    rewrite Nnat.Nat2N.id.
+    auto using Forall2_repeat_r.
+  Qed.
+
+  Lemma type_struct : forall es τs,
+      Forall2 (type_expr Δ Γ) es τs ->
+      `⟨ Δ, Γ ⟩ ⊢ Expr.Lists Expr.lists_struct es ∈ Expr.TStruct false τs.
+  Proof using. eauto. Qed.
+
+  Lemma type_header : forall b es τs,
+      Forall2 (type_expr Δ Γ) es τs ->
+      `⟨ Δ, Γ ⟩ ⊢ Expr.Lists (Expr.lists_header b) es ∈ Expr.TStruct true τs.
+  Proof using. eauto. Qed.
+
+  Local Hint Constructors type_expr : core.
+  
+  Lemma rename_type_expr : forall τs e τ,
+      `⟨ Δ, Γ ⟩ ⊢ e ∈ τ ->
+      `⟨ Δ, τs ++ Γ ⟩
+        ⊢ rename_e (Nat.add (length τs)) e ∈ τ.
+  Proof using.
+    intros ts e t het.
+    induction het using custom_type_expr_ind; unravel in *; eauto.
+    - constructor; auto; unravel.
+      rewrite nth_error_app3; assumption.
+    - econstructor; eauto.
+    - econstructor; eauto.
+      rewrite <- Forall2_map_l; unravel; assumption.
+  Qed.
+
+  Lemma shift_type_expr : forall ts1 ts2 τ e,
+      `⟨ Δ, ts1 ++ Γ ⟩ ⊢ e ∈ τ ->
+      `⟨ Δ, ts1 ++ ts2 ++ Γ ⟩
+        ⊢ shift_e (Shifter (length ts1) (length ts2)) e ∈ τ.
+  Proof using.
+    intros ts1 ts2 t e h.
+    (*generalize dependent ts2.*)
+    remember (ts1 ++ Γ) as TS eqn:hTS.
+    induction h using custom_type_expr_ind;
+      (*intros ts2;*) subst; unravel; eauto.
+    - constructor; auto.
+      unfold shift_var. destruct_if.
+      + assert (length (ts1 ++ ts2) <= length ts2 + x) as h.
+        { rewrite app_length. lia. }
+        rewrite app_assoc.
+        rewrite nth_error_app2 in * by assumption.
+        rewrite app_length.
+        replace (length ts2 + x - (length ts1 + length ts2))
+          with (x - length ts1) by lia.
+        assumption.
+      + rewrite nth_error_app1 in * by assumption.
+        assumption.
+    - econstructor; eauto.
+    - econstructor; eauto.
+      rewrite <- Forall2_map_l; unravel.
+      apply Forall2_dumb in H2; assumption || reflexivity.
+  Qed.
 End Lemmas.
